theories/core/utp_opsem.thy
@@ -1,0 +1,98 @@
+(******************************************************************************)
+(* Project: Unifying Theories of Programming in HOL                           *)
+(* File: utp_opsem.thy                                                        *)
+(* Author: Frank Zeyda, University of York (UK)                               *)
+(******************************************************************************)
+
+header {* Operational Semantics *}
+
+theory utp_opsem
+imports 
+  utp_pred 
+  utp_expr 
+  utp_rename 
+  utp_unrest 
+  utp_rel
+  "../laws/utp_rel_laws"
+  "../laws/utp_refine_laws"
+begin
+
+type_synonym 'a WF_STATE = "('a WF_PREDICATE * 'a WF_PREDICATE)"
+
+fun StepP :: "'a WF_STATE \<Rightarrow> 'a WF_STATE \<Rightarrow> bool" (infix "~>" 50) where
+"(s,P) ~> (t,Q) \<longleftrightarrow> (s\<acute>;P) \<sqsubseteq> (t\<acute>;Q)"
+
+lemma SkipR_step:
+  "(s, II; P) ~> (s, P)"
+  by simp
+
+lemma SeqR_step:
+  "(s,P) ~> (t,P') \<Longrightarrow> (s, P;Q) ~> (t, P';Q)"
+  apply (simp)
+  apply (simp add:SemiR_assoc)
+  apply (rule refine)
+  apply (assumption)
+  apply (rule order_refl)
+done
+
+lemma ChoiceP_step1:
+  "(s, P \<sqinter> Q) ~> (s, P)"
+  apply (simp)
+  apply (metis RefineP_choice1 SemiR_mono_refine order_refl)
+done
+
+lemma ChoiceP_step2:
+  "(s, P \<sqinter> Q) ~> (s, Q)"
+  apply (simp)
+  apply (metis RefineP_choice2 SemiR_mono_refine order_refl)
+done
+
+(*
+lemma 
+  assumes 
+    "P \<in> WF_RELATION" 
+    "Q \<in> WF_RELATION"
+    "- vs \<sharp> P"
+    "- vs \<sharp> Q"
+    "\<And> s t. \<lbrakk> s \<in> WF_ASSIGN vs; t \<in> WF_ASSIGN vs; (s ; P) \<sqsubseteq> t \<rbrakk> \<Longrightarrow> (s ; Q) \<sqsubseteq> t" 
+  shows "P \<sqsubseteq> Q"
+  using assms
+  apply (utp_xrel_auto_tac)
+
+
+lemma 
+  assumes 
+    "s \<in> WF_POSTCOND"
+    "P \<in> WF_RELATION"
+    "Q \<in> WF_RELATION"
+  shows "`s ; (P \<and> Q)` = `(s ; P) \<and> (s ; Q)`"
+  nitpick
+  apply (simp add:closure SemiR_algebraic_rel assms urename)
+proof -
+  have "`s ; (P \<and> Q)` = `true ; (s\<acute> \<and> P \<and> Q)`"
+    by (metis AndP_rel_closure SemiR_AndP_left_postcond TrueP_rel_closure assms(1) assms(2) assms(3) utp_pred_simps(6))
+
+  have "... = `true ; ((s\<acute> \<and> P) \<and> (s\<acute> \<and> Q))`"
+    by (smt AndP_comm AndP_idem AndP_assoc)
+
+  using assms
+  
+
+  apply (frule_tac SemiR_TrueP_postcond)
+  apply (utp_xrel_auto_tac)
+  apply (utp_rel_auto_tac)
+
+lemma CondR_true_step:
+  "[s\<acute>;b] \<Longrightarrow> (s, P \<lhd> b \<rhd> Q) ~> (s, P)"
+  apply (simp add:CondR_def SemiR_OrP_distl)
+  apply (utp_rel_auto_tac)
+  apply (rule refine)
+
+  by (simp)
+
+lemma CondR_false_step:
+  "[\<not>(s\<acute>;b)] \<Longrightarrow> (s, P \<lhd> b \<rhd> Q) ~> (s, Q)"
+  by (simp)
+*)
+
+end
