theories/laws/utp_poly_laws.thy
@@ -11,6 +11,7 @@ imports
   "../poly/utp_poly_expr"
   "../parser/utp_pred_parser"
   utp_pred_laws
+  utp_rel_laws
   utp_rename_laws
   utp_subst_laws
 begin
@@ -24,5 +25,42 @@ lemma BoolType_pvaux_cases [ucases]:
   apply (rule BoolType_aux_var_split_eq_intro[of "x\<down>"])
   apply (simp_all add:typing defined erasure pvaux_aux)
 done
+
+theorem SemiR_extract_variable_ty:
+  fixes x :: "('a :: DEFINED, 'm :: VALUE) PVAR"
+  assumes "P \<in> WF_RELATION" "Q \<in> WF_RELATION"
+          "x \<in> PUNDASHED" "pvaux x"
+          "TYPEUSOUND('a, 'm)"
+  shows "P ; Q = `\<exists> x\<acute>\<acute>\<acute>. P[$x\<acute>\<acute>\<acute>/x\<acute>] ; Q[$x\<acute>\<acute>\<acute>/x]`"
+  apply (subst SemiR_extract_variable[of _ _ "x\<down>"])
+  apply (simp_all add:assms)
+  apply (metis PVAR_VAR_PUNDASHED_UNDASHED assms(3))
+  apply (simp add:erasure assms typing defined closure)
+done
+
+theorem AssignR_SemiR_ty:
+  fixes x :: "('a :: DEFINED, 'm :: VALUE) PVAR"
+  assumes 
+    "TYPEUSOUND('a, 'm)"
+    "x \<in> PUNDASHED" 
+    "e \<rhd>\<^sub>* x" 
+    "DASHED \<sharp> e"
+  shows "`(x := e) ; p` = `p[e/x]`"
+  apply (utp_rel_tac)
+  apply (simp add: EvalR_AssignR_typed evalp closure typing defined unrest relcomp_unfold assms EvalR_SubstP_UNDASHED_ty)
+  apply (auto simp add: binding_upd_ty_def)
+  apply (metis InjU_EvalPE_compat PVAR_VAR_PUNDASHED_UNDASHED WF_REL_BINDING_binding_upd_remove WF_REL_BINDING_member1 assms(2) assms(3))
+done
+
+text {* Declare some useful simplications for polymorphic expressions *}
+
+lemma [simp]: "(x::int) < y \<Longrightarrow> `<x> < <y>` = true"
+  by (simp add:eval)
+
+lemma [simp]: "\<not> (x::int) < y \<Longrightarrow> `<x> < <y>` = false"
+  by (simp add:eval)
+
+lemma [simp]: "|<x :: int> + <y>| = |<x + y>|"
+  by (simp add:evalp)
 
 end
